{"cells":[{"cell_type":"markdown","metadata":{},"source":["### Proof of Sum Rule\n\n"]},{"cell_type":"markdown","metadata":{},"source":["Proof of (d/dx) [f(x) + g(x)] = (d/dx) f(x) + (d/dx) g(x) from the definition.\n\nWe can use the definition of the derivative:\n\n$\\frac{d}{dx} f(x) =\t\\lim_{x\\to 0} \\frac{f(x+d)-f(x)}{d}$\n\nTherefore, $\\frac{d}{dx} [f(x) + g(x)] =\t\\lim_{x\\to 0} \\frac{[f(x+d)+ g(x+d)] - [f(x)+g(x)]}{d}$\n\nLet's just rearrange this a little: $\\frac{[f(x+d) - f(x) ] + [g(x+d) + g(x)]}{d}$, and then $\\frac{f(x+d) - f(x)}{d} + \\frac{g(x+d) + g(x)}{d}$.\n\nBut this is just our original definition.\n\n"]},{"cell_type":"markdown","metadata":{},"source":["### Proof of Chain Rule\n\n"]},{"cell_type":"markdown","metadata":{},"source":["Prime notation shows the mechanics clearer, Leibniz notation the concept.\nPrime notation: $(f o g)' (x) = f'(g(x)) \\cdot g'(x)$\n\nAnd from Leibniz: $\\frac{dy}{dx} = \\frac{dy}{du} \\frac{du}{dx}$\n\nSince we are asking about a rate of change, relative to another rate of change,\nwhich is relative to x, it make sense that any change to x gets amplified as it\nricochets through our little machine.\n\ndy/dx is the result of a function. It is f(x + dx) - f(x) by (x + dx).\nActually, I suppose they are both infinitesimals, but the dy infinitesimal is\nobtained through a function.\n\nThe proof is a straight-up algebraic \"chain\" of reasoning.\n\n"]},{"cell_type":"markdown","metadata":{},"source":["#### Part A\n\n"]},{"cell_type":"markdown","metadata":{},"source":["Remember $\\Delta y = f(a + \\Delta x) - f(x)$, and as $\\Delta x \\rightarrow 0$ we have $\\Delta y/\\Delta x = f'(a)$.\n\nLet's make $\\epsilon$ equal the difference between our [ difference quotient ](https://en.wikipedia.org/wiki/Difference_quotient) and the derivative.\n\nAs $\\Delta x \\rightarrow 0$, we have $\\epsilon = (\\frac{\\Delta y}{\\Delta x} - f'(a)) = f'(a) - f'(a) = 0$.\n\nThis lets us do $\\epsilon = (\\Delta y/\\Delta x - f'(a) \\Rightarrow \\Delta y = f'(a) \\Delta x + \\epsilon \\Delta x$\n\nTo make $\\epsilon$ differentiable, we let it go to 0 when $\\Delta x = 0$.\n$\\Delta y = f'(a) \\Delta x + \\epsilon \\Delta x$ where $\\epsilon \\to 0$ as $\\Delta x \\to 0$.\n\nThis is a little obscurantist, because f'(a) and our difference quotient are exactly\nthe same thing.\n\n"]},{"cell_type":"markdown","metadata":{},"source":["#### Part B\n\n"]},{"cell_type":"markdown","metadata":{},"source":["The stage is now set. Suppose $u = g(x)$ is differentiable at a, and $y = f(u)$ at \nthe same location, but we'll say $b = g(a)$. $f(g(a))$, or $f(b)$.\n\nThen, $\\Delta u = g'(a) \\Delta x + \\epsilon \\Delta x$. And this equals $[g'(a) + \\epsilon](\\Delta x)$.\n\nAnd, $\\Delta y = f'(b) (\\Delta u) + \\epsilon (\\Delta u)$. And, $= [f'(b) + \\epsilon](\\Delta u)$.\n\nSubstituting the first result into the second, we have\n$\\Delta y = [f'(b) + \\epsilon] [g'(a) + \\epsilon](\\Delta x)$.\nNow as $\\Delta x \\to 0$, so does $\\Delta u$, and thus both our $\\epsilon \\to 0$.\nTherefore $\\frac{dy}{dx} = (\\Delta x \\to 0) (\\Delta y)/(\\Delta x) = (lim \\Delta x \\to 0) [f'(b) + \\epsilon] [g'(a) + \\epsilon] = f'(b) g'(a) = f'(g(a)) g'(a)$.\n\n"]},{"cell_type":"markdown","metadata":{},"source":["#### This proves the Chain Rule.\n\n"]},{"cell_type":"markdown","metadata":{},"source":["We found a way to represent the change in y as the result of the derivative of\na point plus a small change, multiplied by the change in x - to show a change in\ny in reference to an already-established rate.\n\nThis somewhat sneaky characterization let us see more clearly what we could not\nbefore - that the change in y relative to the change in x, when functions are composed,\ndepends on the derivatives of both functions.\n\n$\\epsilon = (\\Delta y)/(\\Delta x) - (\\Delta y)/(\\Delta x)$\n\n$\\Delta x \\epsilon = \\Delta y - (\\Delta x)[(\\Delta y)/(\\Delta x)]$\n\n$\\Delta y = (\\Delta x)[(\\Delta y)/(\\Delta x)] + (\\Delta x) \\epsilon$\n\n$\\Delta y = (\\Delta x)[(\\Delta y)/(\\Delta x) + \\epsilon]$\n\n$(\\Delta y)/(\\Delta x) = (\\Delta y)/(\\Delta u) (\\Delta u)/(\\Delta x)$\n\nBut since we are not using infinitesimals, and we use the Leibniz notation because \nsometimes it shows these relations more clearly, we cannot cancel out $(\\Delta u)$.\nRather, these represent the results of taking the limit, and given any actual\nfunctions f and g, we would have to apply our usual method of adding an h and\ndoing algebra, and so on.\n\nSo we can treat $\\Delta x$ and others above as algebraic quantities, but to actually\nfind the derivative we then must find the limit as $\\Delta x \\to 0$. We can work with them\nalgebraically before taking the limit, but not use them to actually find the derivative.\n\n"]}],"metadata":{"org":null,"kernelspec":{"display_name":"Python 3","language":"python","name":"python3"},"language_info":{"codemirror_mode":{"name":"ipython","version":3},"file_extension":".py","mimetype":"text/x-python","name":"python","nbconvert_exporter":"python","pygments_lexer":"ipython3","version":"3.5.2"}},"nbformat":4,"nbformat_minor":0}